\section{$A_5[1^-2^-3^+4^+5^+]^{\mathrm{1-loop}}$ in N=4}
There are four possible configurations contributing to the quadruple cut.
\begin{figure}[h!]
  \centering
    \includegraphics[width=\linewidth]{A5-1}
    \caption{A5-1}
  \label{A5-1}
\end{figure}
Let us now compute the box coefficients.
%
\paragraph{\ref{A5-1}}
The on-shell conditions allow us to set
\begin{equation*}
|l_1\rangle = \alpha |5\rangle \quad
|l_2\rangle = \delta |3\rangle \quad
|l_3\rangle = \gamma |l_3\rangle\quad
|l_3] = \eta|4]\quad
|l_4] = \beta 4]
\end{equation*}
Hence, the coefficient
\begin{equation*}
\begin{split}
c_1 = &
\frac{1}{2}\frac{\langle 12 \rangle^4}{\langle 1 2 \rangle \langle 2 l_2\rangle \langle l_2 l_1 \rangle\langle l_1 1 \rangle}
\frac{[3l_3]^3}{[l_3 l_2][l_2 3]}
\frac{\langle l_3 l_4 \rangle^{3}}{\langle l_4 4 \rangle \langle 4 l_3\rangle}
\frac{[l_4 5 ]^3}{[5l_1][l_1 l_4]}
\\
= & 
\frac{1}{2}\frac{\langle 12 \rangle^3}{\langle 2 l_2 \rangle\langle l_2 l_1 \rangle\langle l_1 1\rangle}
\frac{[34]^2\langle l_4 4\rangle}{[l_3 l_2][l_2 3]\langle 4 l_3\rangle}
\frac{[l_4 5]^2}{[5l_1 ][l_1 l_4]}
[3 l_3]\langle l_3 l_4 \rangle [l_4 5]
\\
= &
\frac{1}{2}
\frac{\langle 12 \rangle^3[34]^2[45]}{\langle 15 \rangle\langle2|\slashed{K}_{3}|4]}
\\
= &
\frac{1}{2}\frac{\langle 12 \rangle^4 s_{34}s_{45}}{\langle 12 \rangle\langle 23 \rangle \langle 34\rangle \langle 45\rangle \langle 51\rangle}
\\
= &
\frac{1}{2}s_{34}s_{45}A_5^{\textrm{MHV-tree}}[12345]
\end{split}
\end{equation*}
As we will see, all the contributions that we will compute are related to the tree-level amplitude by the same structure as given in the last line.   
%
%
%
%%%%%%%%%%%%%%%%%%%%%%%%%%%%%%%
%Not used
%
\iffalse
\begin{figure}[h!]
  \centering
    \includegraphics[width=\linewidth]{A5-2}
    \caption{A5-2}
  \label{A5-2}
\end{figure}
\paragraph{\ref{A5-2}}
%
\begin{equation*}
\begin{split}
c_2  = &
\frac{1}{2}\frac{\langle 21\rangle^4}{\langle 21 \rangle\langle 1l_1\rangle\langle l_1l_2\rangle\langle l_2 2\rangle}
\frac{\langle l_2 l_3\rangle^3}{\langle l_3 3\rangle\langle 3 l_2\rangle}
\frac{[l_3 4]^3}{[4l_4][l_4 l_3]}
\frac{[5 l_4]^3}{[l_4 l_1][l_1 5]}
\\
= &
\frac{1}{2}\frac{\langle 12 \rangle^3[l_4 4 ]^2\langle l_2l_4\rangle^2 [l_4 5]\langle l_2 5\rangle}{\langle 15\rangle\langle 5 l_2 \rangle\langle l_2 2\rangle[l_4 l_2]\langle l_2 3\rangle^2
}
\\
= &
-\frac{1}{2}\frac{\langle 21 \rangle^3}{\langle 1 l_1 \rangle\langle l_1 l_2 \rangle\langle l_2 2 \rangle}
\frac{\langle l_2 3 \rangle^2[34]^3[5l_4]^3}{[l_4 3]\langle 3 4 \rangle [4 l_4][l_4 l_1][l_1 5]}
\\
= & 
\frac{1}{2}
\frac{\langle 21 \rangle^3 \langle l_2 3 \rangle^2 [34]^3 [5l_4]^2}{\langle 1 l_4 \rangle [l_4|\slashed{K}_{12}|l_2\rangle\langle l_2 2 \rangle [l_4 3]\langle 34 \rangle [4l_4]}
\end{split}
\end{equation*}
Due to the on-shell kinematic relations, we can write
\begin{equation*}
|l_3] = \alpha 3] \quad
|l_3\rangle = \beta |4\rangle \quad
|l_4\rangle = c|4\rangle \quad
|l_2] = f |3]
\end{equation*}
We re-express the remaining undetermined terms in using the on-shell conditions
\begin{equation*}
\langle l_3|\slashed{K}_{123}|l_3\rangle = K_{123}^2 \quad\Rightarrow
\alpha\beta \langle 4 | \slashed{K}_{123}|3] = K_{123}^2
\quad\Rightarrow
[4l_4]\langle l_4 1 \rangle = \alpha\beta [43]\langle 41 \rangle
=\frac{K_{123}^2}{\langle 4 |\slashed{K}_{123}|3]}[43]\langle 4 1 \rangle
\end{equation*}
Supposing
\begin{equation*}
|l_4] = a|3] + b|4] \quad
|l_2\rangle = d|3\rangle + e|4\rangle
\end{equation*}
we then have
\begin{equation*}
\begin{split}
&
(l_4 + K_{34})^2 = (l_4 + K_{1234})^2 = 0
\quad\Rightarrow
bc = \frac{K_{34}^2}{[4|\slashed{K}_3}|4\rangle
,\quad
ac = \frac{1}{[3|\slashed{K}_{12}|4\rangle}\Big(K_{1234}^2 - \frac{K_{34}^2 [4|\slashed{K}_{123}|4\rangle}{[4|\slashed{K}_3|4\rangle}\Big)
\\
&
(l_2 + K_{34} )^2 = (l_2 + K_{12})^2= 0 \quad\Rightarrow
df = \frac{K_{34}^2}{[3|\slashed{K}_4|3\rangle}
,\quad
de = \frac{1}{[3 | \slashed{K}_{12}|4\rangle}\Big(K_{12}^2 - \frac{[3|\slashed{K}_{12}|3\rangle K_{34}^2}{[3|\slashed{K}_4|3\rangle}\Big)
\end{split}
\end{equation*}
Since we have the same degree in loop spinors in the numerator and in the denominator, the exact values of $c$ and $f$ are not important.
%
\begin{figure}
  \centering
    \includegraphics[width=\linewidth]{A5-3}
    \caption{A5-3}
  \label{A5-3}
\end{figure}
\paragraph{\ref{A5-3}}
\begin{equation*}
\begin{split}
c_3 = &
\frac{1}{2}
\frac{\langle 12 \rangle^4}{\langle 12 \rangle\langle 2l_2 \rangle\langle l_2 l_1 \rangle\langle l_1 1 \rangle}
\frac{[3l_3]^3}{[l_3 l_2][l_2 3]}
\frac{[4 l_4]^3}{[l_4 l_3][l_3 l_4]}
\frac{\langle l_4 l_1 \rangle^3}{\langle l_4 5\rangle\langle 5 l_1 \rangle}
\\
= &
\frac{1}{2}\frac{\langle 12 \rangle^3 [3|\slashed{K}_{12}|l_1\rangle^2}{\langle 23 \rangle [ 3 l_3]\langle l_1 1\rangle}\frac{[4l_3]}{\langle 45\rangle\langle 5l_1\rangle}
\end{split}
\end{equation*}
Set
\begin{equation*}
|l_1] = \alpha|5] ,\quad
|l_3\rangle = \beta|4\rangle, \quad
|l_1\rangle = a |4\rangle + b|5\rangle ,\quad
|l_3] = c|4] + d|5] 
\end{equation*}
Then
\begin{equation*}
\begin{split}
& (l_1 + K_{45})^2 = (l_1 - K_{12})^2 = 0 \quad\Rightarrow
\alpha b = \frac{-K_{45}^2}{[5|\slashed{K}_4|5\rangle} ,\quad
\alpha a = \frac{1}{[5|\slashed{K}_{12}|4\rangle}\Big(K_{12}^2 + \frac{K_{45}^2[5|\slashed{K}_4|5\rangle}{[5|\slashed{K}_{12}|5\rangle}\Big)
\\
& (l_3 -K_{45})^2 = (l_3 + K_3)^2 = 0 \quad\Rightarrow
\beta c =\frac{K_{45}^2}{[4|\slashed{K}_5|4\rangle} ,\quad
\beta d = \frac{1}{[5|\slashed{K}_3|4\rangle}\Big( -K_3^2 - \frac{K_{45}^2[4|\slashed{K}_3|4\rangle}{[4|\slashed{K}_5|4\rangle}\Big)
\end{split}
\end{equation*}
%
%
\begin{figure}
  \centering
    \includegraphics[width=\linewidth]{A5-4}
    \caption{A5-4}
  \label{A5-4}
\end{figure}
\paragraph{\ref{A5-4}}
\begin{equation*}
\begin{split}
c_4 = & \frac{1}{2}\frac{\langle 12 \rangle^4}{\langle 12 \rangle\langle 2l_2 \rangle\langle l_2 l_1 \rangle\langle l_1 1 \rangle}
\frac{\langle l_2 l_3 \rangle^3}{\langle l_2 3 \rangle \langle 3 l_3 \rangle}
\frac{[l_3 4 ]^3}{[l_4 l_3][4 l_4]}
\frac{[l_4 5]^3}{[5l_1][l_1 l_4]}
\\
= &
-\frac{1}{2}\frac{\langle 12 \rangle^3}{\langle 2l_2\rangle\langle l_2 l_4 \rangle\langle 51 \rangle}
\frac{\langle l_2 3 \rangle^2 [34]^3 [l_4 5]}{\langle 3 l_3 \rangle [l_4 l_3][4 l_4]}
\\
= &
-\frac{\langle 12 \rangle^3\langle l_2 3\rangle^2[34]^3[l_4 5]}{\langle 2 l_2 \rangle\langle l_2 l_4 \rangle\langle 51 \rangle\langle 34 \rangle [l_4 4]^2}
\end{split}
\end{equation*}
Set
\begin{equation*}
|l_2] = \alpha|3] \quad
|l_4\rangle = \beta|4\rangle \quad
|l_4] = a|3] + b|4] \quad
|l_2\rangle = c|3\rangle + d|4\rangle
\end{equation*}
We solve the coefficients with the on-shell conditions
\begin{equation*}
\begin{split}
& (l_4 + K_{34})^2 = (l_4 +K_{1234})^2 = 0 \quad\Rightarrow
b\beta = -\frac{K_{34}^2}{[4|\slashed{K}_3|4\rangle} ,\quad
a\beta = \frac{1}{[3|\slashed{K}_{12}|4\rangle}\Big( -K_{1234}^2 + \frac{K_{34}^2 [4|\slashed{K}_{123}|4\rangle}{[4|\slashed{K}_3|4\rangle}\Big)
\\
&
(l_2 + K_{34})^2 = (l_2 + K_{1234})^2 = 0 \quad\Rightarrow
\alpha c = -\frac{K_{34}^2}{[3|\slashed{K}_4|3\rangle} ,\quad
\alpha d = \frac{1}{[3|\slashed{K}_{12}|4\rangle}\Big(-K_{1234}^2 + \frac{K_{34}^2 [3|\slashed{K}_{124}|3\rangle}{[3|\slashed{K}_4|3\rangle}\Big)
\end{split}
\end{equation*}
%
%
%
\begin{figure}
  \centering
    \includegraphics[width=\linewidth]{A5-5}
    \caption{A5-5}
  \label{A5-5}
\end{figure}
\paragraph{\ref{A5-5}}
\begin{equation*}
\begin{split}
c_5 = & \frac{1}{2}\frac{[l_1 l_2]^3}{[l_2][l_1]}\frac{\langle l_2 3 \rangle^4}{\langle l_2 2 \rangle\langle 23 \rangle\langle 3 l_3 \rangle\langle l_3 l_2\rangle}
\frac{\langle l_3 l_4 \rangle^3}{\langle l_3 4 \rangle\langle 4 l_4 \rangle}
\frac{[l_4 5]^3}{[5 l_1][l_1 l_4]}
\\
= &
\frac{1}{2}\frac{[l_1 1 ]^2 \langle 12 \rangle^3 \langle l_3 4 \rangle^2[45]^3}{\langle 23 \rangle\langle 3 l_3 \rangle\langle l_3 |\slashed{K}_{23}|1]\langle 45 \rangle [5l_1]^2}
\end{split}
\end{equation*}
%
%
\begin{figure}
  \centering
    \includegraphics[width=\linewidth]{A5-6}
    \caption{A5-6}
  \label{A5-6}
\end{figure}
\paragraph{\ref{A5-6}}
\begin{equation*}
\begin{split}
c_6 = & \frac{1}{2}\frac{\langle 1l_1\rangle^3}{\langle l_1 l_2 \rangle\langle l_2 1 \rangle}
\frac{\langle l_2 2 \rangle^4}{\langle l_2 2\rangle\langle 23 \rangle\langle 3l_3\rangle\langle l_3 l_2 \rangle}
\frac{[4l_4]^3}{[l_4 l_3][l_3 4]}
\frac{[5l_1]^3}{[l_1l_4][l_4 5]}
\\
= &
\frac{1}{2}
\frac{\langle l_2 2 \rangle^3\langle 1 l_4\rangle^3[l_4 5][4 l_4]}{\langle 5 l_2 \rangle\langle l_2 1 \rangle\langle 23 \rangle\langle 34 \rangle\langle l_2 l_4 \rangle}
\end{split}
\end{equation*}
%
%
\begin{figure}
  \centering
    \includegraphics[width=\linewidth]{A5-7}
    \caption{A5-7}
  \label{A5-7}
\end{figure}
\paragraph{\ref{A5-7}}
\begin{equation*}
\begin{split}
c_7 = & \frac{1}{2}\frac{\langle 1 l_2 \rangle^3}{\langle l_2 l_1 \rangle\langle l_1 1\rangle}
\frac{\langle 2 l_3 \rangle^4}{\langle 23\rangle\langle 3 l_3 \rangle\langle l_3 l_2\rangle\langle l_2 2 \rangle}
\frac{[l_3 4]^3}{[4 l_4][l_4 l_3]}
\frac{[l_4 5 ]^3}{[5 l_1 ][l_1 l_4]}
\\
= &
-\frac{1}{2}
\frac{\langle 1 l_2 \rangle^2\langle 24 \rangle [l_4 5]^2\langle 2 l_4\rangle^3 [l_4 4]}{[15]\langle 51 \rangle \langle 23 \rangle \langle 34 \rangle\langle l_2 2 \rangle\langle 4 l_2\rangle}
\end{split}
\end{equation*}
where $| l_3\rangle \propto |4\rangle$ is used in the second line.
%
%
\fi %end of the unused block
%%%%%%%%%%%%%
%
\begin{figure}
  \centering
    \includegraphics[width=\linewidth]{A5-8}
    \caption{A5-8}
  \label{A5-8}
\end{figure}
\paragraph{\ref{A5-8}}
\begin{equation*}
\begin{split}
c_8 = & \frac{1}{2}
\frac{[l_1 l_2]^3}{[l_1 1][1l_2]}
\frac{\langle 2 l_2 \rangle^4}{\langle 2l_2 \rangle\langle l_2 l_3\rangle\langle l_3 3 \rangle\langle 32 \rangle}
\frac{[l_4 4 ]^3}{[l_4 l_3][l_3 4]}
\frac{\langle l_4 l_1 \rangle^3}{\langle l_4 5 \rangle\langle 5 l_1\rangle}
\\
= &
\frac{\langle 12 \rangle^3[1l_1 ]\langle l_1 5\rangle^2 [54]^3}{\langle l_1 l_3\rangle\langle l_3 3 \rangle\langle 32 \rangle [l_3 4 ]^2\langle 45\rangle}
\end{split}
\end{equation*}
By the three-particle kinematics, set
\begin{equation*}
|l_1] = \alpha |5]
\quad,\quad
|l_1\rangle = a|4\rangle + b|5\rangle
\quad,\quad
|l_3\rangle = \beta |4\rangle
\quad,\quad
|l_3] = c|4] + d|5]
\end{equation*}
From $(l_1 - K_1)^2 = 0$, we get
\begin{equation*}
a\langle 14\rangle = -b\langle 15 \rangle
\end{equation*}
and from $(l_1 + K_{45})^2 = 0$, we get
\begin{equation*}
K_{45}^2 = -b\alpha [5|\slashed{K}_4|5\rangle 
\end{equation*}
Hence
\begin{equation*}
a\alpha = \frac{\langle 15\rangle}{\langle 14\rangle}\quad,\quad
b\alpha = -1
\end{equation*}
On the other hand
\begin{equation*}
\begin{split}
& (l_3 - K_{45})^2 = 0 \quad\Rightarrow\quad
K_{45}^2 = c\beta [4|\slashed{K}_5|4\rangle
\\
& (l_3 + K_{23})^2 = 0 \quad\Rightarrow\quad
K_{23}^2 = -c\beta [4|\slashed{K_{23}}|4\rangle - d\beta [5|\slashed{K}_{23}|4\rangle
\end{split}
\end{equation*}
Therefore
\begin{equation*}
c\beta = 1 \quad,\quad 
d\beta = \frac{K_{234}^2}{[51]\langle 14 \rangle}
\end{equation*}
Putting all these results back, we get
\begin{equation*}
c_8 = \frac{1}{2} s_{51}s_{45} \frac{\langle 12 \rangle^3 [15] [54]}{\langle 43 \rangle\langle 32 \rangle}=\frac{1}{2} s_{51}s_{45} A_5^{\textrm{MHV-tree}}[12345]
\end{equation*}
%
%
\iffalse % unused block
%
\begin{figure}
  \centering
    \includegraphics[width=\linewidth]{A5-9}
    \caption{A5-9}
  \label{A5-9}
\end{figure}
\paragraph{\ref{A5-9}}
\begin{equation*}
\begin{split}
c_9 = & \frac{1}{2}\frac{[l_1 l_2]^3}{[l_1 1][1 l_2]}
\frac{\langle 2l_2 \rangle^3}{\langle l_2 l_3 \rangle\langle l_3 2 \rangle}
\frac{[34]^4}{[34][4 l_4][l_4 l_3][l_3 3]}
\frac{[l_4 5]^3}{[l_4 l_1][l_1 5]}
\\
= &
-\frac{1}{2}
\frac{\langle 21 \rangle^3 [1l_1]^2[34]^3[l_4 5]^3}{[12][l_4|\slashed{K}_{34}|2\rangle \big(\rangle 2 | \slashed{K}_{24}|3]\big) [4l_4][l_4 l_1 ][l_1 5]}
\end{split}
\end{equation*}
%
\fi %end
%
\begin{figure}
  \centering
    \includegraphics[width=\linewidth]{A5-10}
    \caption{A5-10}
  \label{A5-10}
\end{figure}
\paragraph{\ref{A5-10}}
\begin{equation*}
\begin{split}
c_{10} = &
\frac{1}{2}\frac{\langle 1l_2\rangle^3}{\langle l_2 l_1 \rangle\langle l_1 1 \rangle}
\frac{[l_2 l_3]^3}{[l_2 2 ][2 l_3]}
\frac{[34]^4}{[34][4 l_4][l_4 l_3][l_3 3]}
\frac{[l_4 5]^3}{[l_4 l_1][l_1 5]}
\\
= &
\frac{1}{2}\frac{\langle 12 \rangle^3[2l_3]^3[34]^3[l_4 5 ]^2}{\langle 51 \rangle[15][2l_3]^2\langle l_3 1\rangle [4 l_4][l_4 l_3][l_3 3]}
\end{split}
\end{equation*}
Set
\begin{equation*}
|l_3\rangle = \alpha |2\rangle \quad,\quad |l_3] = a|2] + b|5]
|l_4\rangle = \beta |5\rangle \quad,\quad |l_4] = c|2]+d|5]
\end{equation*}
Then
\begin{equation*}
\begin{split}
& (l_3 + K_{12})^2 = 0 \quad\Rightarrow\quad K_{12}^2 = - \alpha a [2|\slashed{K}_{12}|2\rangle - \alpha b [5|\slashed{K}_{12}|2\rangle
\\
& (l_3 - K_{34})^2 = 0 \quad\Rightarrow\quad K_{34}^2 = \alpha a [2|\slashed{K}_{34}|2\rangle + \alpha b [5|\slashed{K}_{34}|2\rangle
\end{split}
\end{equation*}
which leads to
\begin{equation*}
\alpha a = \frac{[5|\slashed{K}_{34}|5\rangle}{[25]\langle 52\rangle}
\\
\alpha b = \frac{[21]\langle 15\rangle}{[52]\langle 25\rangle}
\end{equation*}
On the other hand
\begin{equation*}
\begin{split}
& (l_4 - K_{45})^2 = 0 \quad\Rightarrow\quad
K_{15}^2 = \beta c[2|\slashed{K}_1|5\rangle + \beta d [5|\slashed{K}_1|5\rangle
\\
& (l_4 + K_{34})^2 = 0 \quad\Rightarrow\quad
K_{34}^2 = \beta c [2|\slashed{K}_1|5\rangle - \beta d [5|\slashed{K}_{34}|5\rangle
\end{split}
\end{equation*}
gives
\begin{equation*}
\beta c = - \frac{[51]\langle 12 \rangle}{[52]\langle 25 \rangle}
\quad,\quad
\beta d = - \frac{[2| \slashed{K}_{34}|2\rangle}{[5|\slashed{K}_2|5\rangle}
\end{equation*}
The coefficient $c_{10}$ is then given by
\begin{equation*}
c_{10} = 
\frac{1}{2}\frac{[21][34]^3[51]\langle 12\rangle^4 [52]^2 \langle 52\rangle[25]}{\big(-[42][51]\langle 12\rangle - [2|\slashed{K}_{34}|2\rangle [45]\big)
\big( K_{51}^2 K_{21}^2 - (2K_2\cdot K_{34})(2K_5\cdot K_{34})\big)
\big( [5|\slashed{K}_{34}|5\rangle [23] - [21]\langle 15\rangle [35]\big)
}
\end{equation*}
Using Schouten identity and the momentum conservation, we can rewrite the terms in the denominator in a more compact way
\begin{equation*}
\begin{split}
& -[42][51]\langle 12\rangle - [2|\slashed{K}_{34}|2\rangle [45] = 
-\langle 32\rangle[52][34]
\\
& K_{51}^2 K_{21}^2 - (2K_2\cdot K_{34})(2K_5\cdot K_{34}) = 
-s_{52}s_{34}
\\
& [5|\slashed{K}_{34}|5\rangle [23] - [21]\langle 15\rangle [35]
= -\langle 45\rangle[52][34]
\end{split}
\end{equation*}
As a result
\begin{equation*}
c_{10} = \frac{1}{2}s_{51}s_{12}A_5^{\textrm{MHV-tree}}[12345]
\end{equation*}
%
%
\begin{figure}
  \centering
    \includegraphics[width=\linewidth]{A5-11}
    \caption{A5-11}
  \label{A5-11}
\end{figure}
\paragraph{\ref{A5-11}}
\begin{equation*}
\begin{split}
c_{11} = &
\frac{1}{2}\frac{[l_1 l_2]^3}{[l_1 1][1l_2]}
\frac{\langle l_2 2 \rangle^3}{\langle 2 l_3 \rangle\langle l_3 l_2 \rangle}
\frac{[3l_4]^3}{[l_4 l_3][l_3 3]}
\frac{[45]^4}{[45][5l_1][l_1l_4][l_4 4]}
\\
= &
-\frac{1}{2}
\frac{[l_1 1]\langle 12 \rangle^3[3l_4]^2[45]^3}{[23]\langle l_1 2 \rangle\langle 23 \rangle[5l_1][l_1l_4][l_4 4]}
\end{split}
\end{equation*}
%
Set
\begin{equation*}
|l_1\rangle = \alpha| 1\rangle \quad,\quad
|l_1] = a|1] + b|3] \quad,\quad
|l_4\rangle = \beta|3\rangle 
| l_4] = c|1] + d|3]
\end{equation*}
Then
\begin{equation*}
\begin{split}
& (l_1- K_{12})^2 = 0 \quad\Rightarrow\quad K_{12}^2 = \alpha a [1|\slashed{K}_2|1\rangle + \alpha b [3|\slashed{K}_2|1\rangle
\\
& (l_1 + K_{45})^2 = 0 \quad\Rightarrow\quad
K_{45}^2 = -\alpha a [1|\slashed{K}_{45}|1\rangle - \alpha b [3|\slashed{K}_{45}|1\rangle
\end{split}
\end{equation*}
so
\begin{equation*}
\alpha a = \frac{[3|\slashed{K}_{12}|3\rangle}{[13]\langle 31\rangle}
\quad,\quad
\alpha b = \frac{[21]\langle 23\rangle}{[13]\langle 31\rangle}
\end{equation*}
On the other hand
\begin{equation*}
\begin{split}
& (l_4 + K_{23})^2 = 0 \quad\Rightarrow\quad K_{23}^2 = -\beta c[1|\slashed{K}_2|3\rangle - \beta d [3|\slashed{K}_2|3\rangle
\\
& (l_4 - K_{45})^2 = 0 \quad\Rightarrow\quad K_{45}^2 = \beta c [1|\slashed{K}_{45}|3\rangle + \beta d [3|\slashed{K}_{45}|3\rangle
\end{split}
\end{equation*}
Hence
\begin{equation*}
\beta c = \frac{[32]\langle 21\rangle}{[31]\langle 13\rangle}
\quad,\quad
\beta d = -\frac{[1|\slashed{K}_{23}|1\rangle}{[31]\langle 13\rangle}
\end{equation*}
and
\begin{equation*}
c_{11} = \frac{1}{2}\frac{[32][21][31]^4\langle 13\rangle\langle 12 \rangle^4 [45]^3}{\big( [3|\slashed{K}_{12}|3\rangle [51] + [21]\langle 23\rangle [53]\big)
\big( [32]\langle 21\rangle[14] - [1|\slashed{K}_{23}|1\rangle[34]\big)
\big( (2K_{12}\cdot K_3)(2K_{23}\cdot K_1) - K_{23}^2K_{21}^2\big)
}
\end{equation*}
Again, using Schouten identity and momentum conservation, we obtain the following equations which simplify the denominator
\begin{equation*}
\begin{split}
& [3|\slashed{K}_{12}|3\rangle [51] + [21]\langle 23\rangle [53] = -[31][54]\langle 43 \rangle 
\\
& -[13][45]\langle 51 \rangle
\\
&
(2K_{12}\cdot K_3)(2K_{23}\cdot K_1) - K_{23}^2K_{21}^2 = s_{45}s_{31}
\end{split}
\end{equation*}
At the end
\begin{equation*}
c_{11} = \frac{1}{2}s_{12}s_{23}A_5^{\textrm{MHV-tree}}[12345]
\end{equation*}
%
%
\begin{figure}
  \centering
    \includegraphics[width=\linewidth]{A5-16}
    \caption{A5-16}
  \label{A5-16}
\end{figure}
\paragraph{\ref{A5-16}}
\begin{equation*}
\begin{split}
c_{16} = & \frac{1}{2}
\frac{\langle l_2 1 \rangle^4}{\langle l_2 1 \rangle\langle 15 \rangle\langle 5 l_1 \rangle\langle l_1 l_2\rangle}
\frac{[l_2 l_3]^3}{[l_3 2 ][2 l_2]}
\frac{\langle l_3 l_4\rangle^3}{\langle l_3 3\rangle\langle 3 l_4\rangle}
\frac{[l_4 4 ]^3}{[4l_1][l_1l_4]}
\\
= & 
-\frac{1}{2}\frac{\langle l_2 1\rangle^3[l_2 2 ]\langle 23 \rangle^3[34]^3}{\langle 15 \rangle[4l_4]\langle l_4 l_2\rangle\langle 3l_2\rangle \langle 3 l_4\rangle\langle 54\rangle[4l_4]}
\end{split}
\end{equation*}
Set
\begin{equation*}
|l_2\rangle = \alpha|2\rangle \quad,\quad
|l_2] = a|2] + b|4] \quad,\quad
|l_4\rangle = \beta |4\rangle \quad,\quad
|l_4] = \gamma|3]
\end{equation*}
Then
\begin{equation*}
\begin{split}
& (l_2 - K_{23})^2 = 0 \quad\Rightarrow\quad K_{23}^2 = \alpha a [2|\slashed{K}_3|2\rangle + \alpha b [4|\slashed{K}_{23}|2\langle
\\
& (l_2 + K_{15})^2 = 0 \quad\Rightarrow\quad K_{15}^2 = -\alpha a [2|\slashed{K}_{15}|2\rangle - \alpha b [4|\slashed{K}_{15}|2\rangle
\end{split}
\end{equation*}
\begin{equation*}
\begin{split}
& \alpha a = \frac{[4|\slashed{K}_{23}|4\rangle}{[24]\langle 42\rangle}
\\
& \alpha b = \frac{[32]\langle 34\rangle}{[24]\langle 42\rangle}
\end{split}
\end{equation*}
On the other hand
\begin{equation*}
(l_4 + K_{23})^2 = 0 \quad,\quad \beta\gamma = \frac{\langle 32\rangle}{\langle 24\rangle}
\end{equation*}
Thus
\begin{equation*}
c_{16}= \frac{1}{2}\frac{\langle 21\rangle^3[34][32]}{\langle 15\rangle\langle 54\rangle} = \frac{1}{2}s_{23}s_{34}A_5^{\textrm{MHV-tree}}[12345]
\end{equation*}

















