\section{Detailed computation for~\cref{remaining_a5}}\label{appendix-a5mhv}
\paragraph{Configuration $c_{8}$}
By~\cref{box_coeff}, the box coefficient corresponding to this configuration is
\begin{equation}
\begin{split}
c_8 = & \frac{1}{2}
\frac{[l_1 l_2]^3}{[l_1 1][1l_2]}
\frac{\langle 2 l_2 \rangle^4}{\langle 2l_2 \rangle\langle l_2 l_3\rangle\langle l_3 3 \rangle\langle 32 \rangle}
\frac{[l_4 4 ]^3}{[l_4 l_3][l_3 4]}
\frac{\langle l_4 l_1 \rangle^3}{\langle l_4 5 \rangle\langle 5 l_1\rangle}
\\
= &
\frac{\langle 12 \rangle^3[1l_1 ]\langle l_1 5\rangle^2 [54]^3}{\langle l_1 l_3\rangle\langle l_3 3 \rangle\langle 32 \rangle [l_3 4 ]^2\langle 45\rangle}
\end{split}
\end{equation}
By the three-particle kinematics and the fact that spinors are two-dimensional objects, set
\begin{equation}\label{coef_c8}
|l_1] = \alpha |5]
\quad,\quad
|l_1\rangle = a|4\rangle + b|5\rangle
\quad,\quad
|l_3\rangle = \beta |4\rangle
\quad,\quad
|l_3] = c|4] + d|5]
\end{equation}
From the on-shell condition $(l_1 - K_1)^2 = 0$, we get
\begin{equation}
a\langle 14\rangle = -b\langle 15 \rangle
\end{equation}
and from another on-shell condition $(l_1 + K_{45})^2 = 0$, we get
\begin{equation}
K_{45}^2 = -b\alpha [5|\slashed{K}_4|5\rangle 
\end{equation}
Hence
\begin{equation}
a\alpha = \frac{\langle 15\rangle}{\langle 14\rangle}\quad,\quad
b\alpha = -1
\end{equation}
In the same manner, we determine the other coeffients in~\cref{coef_c8} by two other on-shell conditions:
\begin{equation}
\begin{split}
& (l_3 - K_{45})^2 = 0 \quad\Rightarrow\quad
K_{45}^2 = c\beta [4|\slashed{K}_5|4\rangle
\\
& (l_3 + K_{23})^2 = 0 \quad\Rightarrow\quad
K_{23}^2 = -c\beta [4|\slashed{K_{23}}|4\rangle - d\beta [5|\slashed{K}_{23}|4\rangle
\end{split}
\end{equation}
Therefore
\begin{equation}
c\beta = 1 \quad,\quad 
d\beta = \frac{K_{234}^2}{[51]\langle 14 \rangle}
\end{equation}
Putting all these results back, we get
\begin{equation}
c_8 = \frac{1}{2} s_{51}s_{45} \frac{\langle 12 \rangle^3 [15] [54]}{\langle 43 \rangle\langle 32 \rangle}=\frac{1}{2} s_{51}s_{45} A_5^{\textrm{MHV-tree}}[12345]
\end{equation}
We will be using this machinery to determine the rest of the coefficients.
%
\paragraph{Configuration $c_{10}$}
\begin{equation}
\begin{split}
c_{10} = &
\frac{1}{2}\frac{\langle 1l_2\rangle^3}{\langle l_2 l_1 \rangle\langle l_1 1 \rangle}
\frac{[l_2 l_3]^3}{[l_2 2 ][2 l_3]}
\frac{[34]^4}{[34][4 l_4][l_4 l_3][l_3 3]}
\frac{[l_4 5]^3}{[l_4 l_1][l_1 5]}
\\
= &
\frac{1}{2}\frac{\langle 12 \rangle^3[2l_3]^3[34]^3[l_4 5 ]^2}{\langle 51 \rangle[15][2l_3]^2\langle l_3 1\rangle [4 l_4][l_4 l_3][l_3 3]}
\end{split}
\end{equation}
Set
\begin{equation}
|l_3\rangle = \alpha |2\rangle \quad,\quad |l_3] = a|2] + b|5]
\quad,\quad
|l_4\rangle = \beta |5\rangle \quad,\quad |l_4] = c|2]+d|5]
\end{equation}
Then
\begin{equation}
\begin{split}
& (l_3 + K_{12})^2 = 0 \quad\Rightarrow\quad K_{12}^2 = - \alpha a [2|\slashed{K}_{12}|2\rangle - \alpha b [5|\slashed{K}_{12}|2\rangle
\\
& (l_3 - K_{34})^2 = 0 \quad\Rightarrow\quad K_{34}^2 = \alpha a [2|\slashed{K}_{34}|2\rangle + \alpha b [5|\slashed{K}_{34}|2\rangle
\end{split}
\end{equation}
which leads to
\begin{equation}
\alpha a = \frac{[5|\slashed{K}_{34}|5\rangle}{[25]\langle 52\rangle}
\\
\alpha b = \frac{[21]\langle 15\rangle}{[52]\langle 25\rangle}
\end{equation}
On the other hand
\begin{equation}
\begin{split}
& (l_4 - K_{45})^2 = 0 \quad\Rightarrow\quad
K_{15}^2 = \beta c[2|\slashed{K}_1|5\rangle + \beta d [5|\slashed{K}_1|5\rangle
\\
& (l_4 + K_{34})^2 = 0 \quad\Rightarrow\quad
K_{34}^2 = \beta c [2|\slashed{K}_1|5\rangle - \beta d [5|\slashed{K}_{34}|5\rangle
\end{split}
\end{equation}
gives
\begin{equation}
\beta c = - \frac{[51]\langle 12 \rangle}{[52]\langle 25 \rangle}
\quad,\quad
\beta d = - \frac{[2| \slashed{K}_{34}|2\rangle}{[5|\slashed{K}_2|5\rangle}
\end{equation}
The coefficient $c_{10}$ is then given by
\begin{equation}
c_{10} = 
\frac{1}{2}\frac{[21][34]^3[51]\langle 12\rangle^4 [52]^2 \langle 52\rangle[25]}{\big(-[42][51]\langle 12\rangle - [2|\slashed{K}_{34}|2\rangle [45]\big)
\big( K_{51}^2 K_{21}^2 - (2K_2\cdot K_{34})(2K_5\cdot K_{34})\big)
\big( [5|\slashed{K}_{34}|5\rangle [23] - [21]\langle 15\rangle [35]\big)
}
\end{equation}
Using Schouten identity and the momentum conservation, we can rewrite the terms in the denominator in a more compact way
\begin{equation}
\begin{split}
& -[42][51]\langle 12\rangle - [2|\slashed{K}_{34}|2\rangle [45] = 
-\langle 32\rangle[52][34]
\\
& K_{51}^2 K_{21}^2 - (2K_2\cdot K_{34})(2K_5\cdot K_{34}) = 
-s_{52}s_{34}
\\
& [5|\slashed{K}_{34}|5\rangle [23] - [21]\langle 15\rangle [35]
= -\langle 45\rangle[52][34]
\end{split}
\end{equation}
As a result
\begin{equation}
c_{10} = \frac{1}{2}s_{51}s_{12}A_5^{\textrm{MHV-tree}}[12345]
\end{equation}
%
\paragraph{Configuration $c_{11}$}
\begin{equation}
\begin{split}
c_{11} = &
\frac{1}{2}\frac{[l_1 l_2]^3}{[l_1 1][1l_2]}
\frac{\langle l_2 2 \rangle^3}{\langle 2 l_3 \rangle\langle l_3 l_2 \rangle}
\frac{[3l_4]^3}{[l_4 l_3][l_3 3]}
\frac{[45]^4}{[45][5l_1][l_1l_4][l_4 4]}
\\
= &
-\frac{1}{2}
\frac{[l_1 1]\langle 12 \rangle^3[3l_4]^2[45]^3}{[23]\langle l_1 2 \rangle\langle 23 \rangle[5l_1][l_1l_4][l_4 4]}
\end{split}
\end{equation}
%
Set
\begin{equation}
|l_1\rangle = \alpha| 1\rangle \quad,\quad
|l_1] = a|1] + b|3] \quad,\quad
|l_4\rangle = \beta|3\rangle 
| l_4] = c|1] + d|3]
\end{equation}
Then
\begin{equation}
\begin{split}
& (l_1- K_{12})^2 = 0 \quad\Rightarrow\quad K_{12}^2 = \alpha a [1|\slashed{K}_2|1\rangle + \alpha b [3|\slashed{K}_2|1\rangle
\\
& (l_1 + K_{45})^2 = 0 \quad\Rightarrow\quad
K_{45}^2 = -\alpha a [1|\slashed{K}_{45}|1\rangle - \alpha b [3|\slashed{K}_{45}|1\rangle
\end{split}
\end{equation}
so
\begin{equation}
\alpha a = \frac{[3|\slashed{K}_{12}|3\rangle}{[13]\langle 31\rangle}
\quad,\quad
\alpha b = \frac{[21]\langle 23\rangle}{[13]\langle 31\rangle}
\end{equation}
On the other hand
\begin{equation}
\begin{split}
& (l_4 + K_{23})^2 = 0 \quad\Rightarrow\quad K_{23}^2 = -\beta c[1|\slashed{K}_2|3\rangle - \beta d [3|\slashed{K}_2|3\rangle
\\
& (l_4 - K_{45})^2 = 0 \quad\Rightarrow\quad K_{45}^2 = \beta c [1|\slashed{K}_{45}|3\rangle + \beta d [3|\slashed{K}_{45}|3\rangle
\end{split}
\end{equation}
Hence
\begin{equation}
\beta c = \frac{[32]\langle 21\rangle}{[31]\langle 13\rangle}
\quad,\quad
\beta d = -\frac{[1|\slashed{K}_{23}|1\rangle}{[31]\langle 13\rangle}
\end{equation}
and
\begin{equation}
c_{11} = \frac{1}{2}\frac{[32][21][31]^4\langle 13\rangle\langle 12 \rangle^4 [45]^3}{\big( [3|\slashed{K}_{12}|3\rangle [51] + [21]\langle 23\rangle [53]\big)
\big( [32]\langle 21\rangle[14] - [1|\slashed{K}_{23}|1\rangle[34]\big)
\big( (2K_{12}\cdot K_3)(2K_{23}\cdot K_1) - K_{23}^2K_{21}^2\big)
}
\end{equation}
Again, using Schouten identity and momentum conservation, we obtain the following equations which simplify the denominator
\begin{equation}
\begin{split}
& [3|\slashed{K}_{12}|3\rangle [51] + [21]\langle 23\rangle [53] = -[31][54]\langle 43 \rangle 
\\
& [32]\langle 21\rangle[14] - [1|\slashed{K}_{23}|1\rangle[34] = -[13][45]\langle 51 \rangle
\\
&
(2K_{12}\cdot K_3)(2K_{23}\cdot K_1) - K_{23}^2K_{21}^2 = s_{45}s_{31}
\end{split}
\end{equation}
At the end
\begin{equation}
c_{11} = \frac{1}{2}s_{12}s_{23}A_5^{\textrm{MHV-tree}}[12345]
\end{equation}
%
%
\paragraph{Configuration $c_{16}$}
\begin{equation}
\begin{split}
c_{16} = & \frac{1}{2}
\frac{\langle l_2 1 \rangle^4}{\langle l_2 1 \rangle\langle 15 \rangle\langle 5 l_1 \rangle\langle l_1 l_2\rangle}
\frac{[l_2 l_3]^3}{[l_3 2 ][2 l_2]}
\frac{\langle l_3 l_4\rangle^3}{\langle l_3 3\rangle\langle 3 l_4\rangle}
\frac{[l_4 4 ]^3}{[4l_1][l_1l_4]}
\\
= & 
-\frac{1}{2}\frac{\langle l_2 1\rangle^3[l_2 2 ]\langle 23 \rangle^3[34]^3}{\langle 15 \rangle[4l_4]\langle l_4 l_2\rangle\langle 3l_2\rangle \langle 3 l_4\rangle\langle 54\rangle[4l_4]}
\end{split}
\end{equation}
Set
\begin{equation}
|l_2\rangle = \alpha|2\rangle \quad,\quad
|l_2] = a|2] + b|4] \quad,\quad
|l_4\rangle = \beta |4\rangle \quad,\quad
|l_4] = \gamma|3]
\end{equation}
Then
\begin{equation}
\begin{split}
& (l_2 - K_{23})^2 = 0 \quad\Rightarrow\quad K_{23}^2 = \alpha a [2|\slashed{K}_3|2\rangle + \alpha b [4|\slashed{K}_{23}|2\rangle
\\
& (l_2 + K_{15})^2 = 0 \quad\Rightarrow\quad K_{15}^2 = -\alpha a [2|\slashed{K}_{15}|2\rangle - \alpha b [4|\slashed{K}_{15}|2\rangle
\end{split}
\end{equation}
\begin{equation}
\begin{split}
& \alpha a = \frac{[4|\slashed{K}_{23}|4\rangle}{[24]\langle 42\rangle}
\\
& \alpha b = \frac{[32]\langle 34\rangle}{[24]\langle 42\rangle}
\end{split}
\end{equation}
On the other hand
\begin{equation}
(l_4 + K_{23})^2 = 0 \quad,\quad \beta\gamma = \frac{\langle 32\rangle}{\langle 24\rangle}
\end{equation}
Thus
\begin{equation}
c_{16}= \frac{1}{2}\frac{\langle 21\rangle^3[34][32]}{\langle 15\rangle\langle 54\rangle} = \frac{1}{2}s_{23}s_{34}A_5^{\textrm{MHV-tree}}[12345]
\end{equation}